Введём вспомогательные обозначения:
$$w_{i} = \frac{x_{i} - \overline{x}}{\sum_{j=1}^{n}(x_{j}-\overline{x})^2}, i = \overline{1,n}$$
$$\hat{b} = \sum_{i=1}^{n} w_{i}y_{i} $$
Некоторые преобразования данных обозначений:
$\sum_{i=1}^{n}w_{i} = 0, \qquad\sum_{i=1}^{n}w_{i}x_{i} = \sum_{i=1}^{n}w_{i}(x_{i}-\bar{x}) =1$ 
$\sum_{i=1}^{n}w_{i}^2 = \sum_{i=1}^{n} \frac{(x_{i}-\bar{x})^2}{\left[ \sum_{j=1}^{n}(x_{j}-\bar{x})^2 \right]^2} = \frac{1}\sum_{j=1}^{n}{(x_{j}-\bar{x})^2}$

**<font color="#d99694">СВОЙСТВА</font>** 

1. $\hat{a}, \hat{b}$ линейны относительно $y_{1},\dots,y_{n}$
> $\hat{b} = \sum_{i=1}^{n}w_{i}y_{i}$
> $\hat{a} = \bar{y} - \hat{b}\bar{x}=\frac{1}{n}\sum_{i=1}^{n}y_{i}-\bar{x}\sum_{i=1}^{n}w_{i}y_{i}=\sum_{i=1}^{n}(\frac{1}{n}-\bar{x}w_{i})y_{i}$


2. $\hat{a},\hat{b}$ - несмещённые оценки a,b
>$\hat{b} = \sum_{i=1}^{n}w_{i}y_{i}=\sum_{i=1}^{n}w_{i}(a+bx_{i}+\epsilon_{i})=a\cancelto{0}{\sum_{i=1}^{n}w_{i}}+b\cancelto{1}{\sum_{i=1}^{n}w_{i}x_{i}}+$$+\sum_{i=1}^{n}\epsilon_{i}w_{i}=b+\sum_{i=1}^{n}w_{i\epsilon_{i}}$
>$\mathbb{M}\hat{b}=b+\sum_{i=1}^{n}w_{i}\cancelto{0}{\mathbb{M}\epsilon_{i}}=b$
>$\hat{a}=\sum_{i=1}^{n}\left( \frac{1}{n}-\bar{x}w_{i} \right)y_{i}=\sum_{i=1}^{n}\left( \frac{1}{n}-\bar{x}w_{i} \right)(a+bx_{i}+\epsilon_{i})=\sum_{i=1}^{n}\left( \frac{1}{n} \right)(a+bx_{i})+$$+\sum_{i=1}^{n}\left( \frac{1}{n}-\bar{x}w_{i} \right)\epsilon_{i}=a+b\bar{x}-a\bar{x}\cancelto{0}{\sum_{i=1}^{n}w_{i}}-b\bar{x}\cancelto{1}{\sum_{i=1}^{n}w_{i}x_{i}}+\sum_{i=1}^{n}\left( \frac{1}{n}-\bar{x}w_{i} \right)\epsilon_{i}$
>$\mathbb{M}\hat{a}=a+\sum_{i=1}^{n}(\frac{1}{n}-\bar{x}w_{i})\cancelto{0}{\mathbb{M}\epsilon_{i}}=a$

>[!INFO] сумма
>$\sum_{i=1}^{n}x_{i}$


